src/Init/Prelude.lean
@@ -1904,7 +1904,7 @@ instance : DecidableEq (BitVec n) := BitVec.decEq
 
 /-- The `BitVec` with value `i`, given a proof that `i < 2^n`. -/
 @[match_pattern]
-protected def BitVec.ofNatLt {n : Nat} (i : Nat) (p : LT.lt i (hPow 2 n)) : BitVec n where
+protected def BitVec.ofNatLT {n : Nat} (i : Nat) (p : LT.lt i (hPow 2 n)) : BitVec n where
   toFin := ⟨i, p⟩
 
 /-- Given a bitvector `x`, return the underlying `Nat`. This is O(1) because `BitVec` is a
@@ -1940,7 +1940,7 @@ This function is overridden with a native implementation.
 -/
 @[extern "lean_uint8_of_nat"]
 def UInt8.ofNatCore (n : @& Nat) (h : LT.lt n UInt8.size) : UInt8 where
-  toBitVec := BitVec.ofNatLt n h
+  toBitVec := BitVec.ofNatLT n h
 
 set_option bootstrap.genMatcherCode false in
 /--
@@ -1981,7 +1981,7 @@ This function is overridden with a native implementation.
 -/
 @[extern "lean_uint16_of_nat"]
 def UInt16.ofNatCore (n : @& Nat) (h : LT.lt n UInt16.size) : UInt16 where
-  toBitVec := BitVec.ofNatLt n h
+  toBitVec := BitVec.ofNatLT n h
 
 set_option bootstrap.genMatcherCode false in
 /--
@@ -2022,7 +2022,7 @@ This function is overridden with a native implementation.
 -/
 @[extern "lean_uint32_of_nat"]
 def UInt32.ofNatCore (n : @& Nat) (h : LT.lt n UInt32.size) : UInt32 where
-  toBitVec := BitVec.ofNatLt n h
+  toBitVec := BitVec.ofNatLT n h
 
 /--
 Unpack a `UInt32` as a `Nat`.
@@ -2094,7 +2094,7 @@ This function is overridden with a native implementation.
 -/
 @[extern "lean_uint64_of_nat"]
 def UInt64.ofNatCore (n : @& Nat) (h : LT.lt n UInt64.size) : UInt64 where
-  toBitVec := BitVec.ofNatLt n h
+  toBitVec := BitVec.ofNatLT n h
 
 set_option bootstrap.genMatcherCode false in
 /--
@@ -2149,7 +2149,7 @@ This function is overridden with a native implementation.
 -/
 @[extern "lean_usize_of_nat"]
 def USize.ofNatCore (n : @& Nat) (h : LT.lt n USize.size) : USize where
-  toBitVec := BitVec.ofNatLt n h
+  toBitVec := BitVec.ofNatLT n h
 
 set_option bootstrap.genMatcherCode false in
 /--
@@ -2201,7 +2201,7 @@ This function is overridden with a native implementation.
 -/
 @[extern "lean_uint32_of_nat"]
 def Char.ofNatAux (n : @& Nat) (h : n.isValidChar) : Char :=
-  { val := ⟨BitVec.ofNatLt n (isValidChar_UInt32 h)⟩, valid := h }
+  { val := ⟨BitVec.ofNatLT n (isValidChar_UInt32 h)⟩, valid := h }
 
 /--
 Convert a `Nat` into a `Char`. If the `Nat` does not encode a valid unicode scalar value,
@@ -2211,7 +2211,7 @@ Convert a `Nat` into a `Char`. If the `Nat` does not encode a valid unicode scal
 def Char.ofNat (n : Nat) : Char :=
   dite (n.isValidChar)
     (fun h => Char.ofNatAux n h)
-    (fun _ => { val := ⟨BitVec.ofNatLt 0 (of_decide_eq_true rfl)⟩, valid := Or.inl (of_decide_eq_true rfl) })
+    (fun _ => { val := ⟨BitVec.ofNatLT 0 (of_decide_eq_true rfl)⟩, valid := Or.inl (of_decide_eq_true rfl) })
 
 theorem Char.eq_of_val_eq : ∀ {c d : Char}, Eq c.val d.val → Eq c d
   | ⟨_, _⟩, ⟨_, _⟩, rfl => rfl
